Java/src/Java/Func/JavaFunc.v
@@ -1,0 +1,379 @@
+Require Import Charge.Open.Subst.
+Require Import Charge.Open.Open.
+Require Import Charge.Open.Stack.
+Require Import Charge.Logics.BILogic.
+Require Import Charge.ModularFunc.ILogicFunc.
+Require Import Charge.ModularFunc.BILogicFunc.
+Require Import Charge.ModularFunc.LaterFunc.
+Require Import Charge.ModularFunc.BaseFunc.
+Require Import Charge.ModularFunc.ListFunc.
+Require Import Charge.ModularFunc.OpenFunc.
+Require Import Charge.ModularFunc.EmbedFunc.
+
+Require Import ExtLib.Core.RelDec.
+Require Import ExtLib.Data.Fun.
+Require Import ExtLib.Data.String.
+Require Import ExtLib.Data.Sum.
+Require Import ExtLib.Tactics.Consider.
+
+Require Import MirrorCore.TypesI.
+Require Import MirrorCore.SymI.
+Require Import MirrorCore.Lemma.
+Require Import MirrorCore.Lambda.Expr.
+Require Import MirrorCore.syms.SymEnv.
+Require Import MirrorCore.syms.SymSum.
+Require Import MirrorCore.Subst.FMapSubst.
+
+Require Import Java.Logic.AssertionLogic.
+Require Import Java.Logic.SpecLogic.
+Require Import Java.Language.Lang.
+Require Import Java.Language.Program.
+Require Import Java.Semantics.OperationalSemantics.
+Require Import Java.Func.JavaType.
+
+Require Import Coq.Strings.String.
+Require Import Coq.Bool.Bool.
+
+Set Implicit Arguments.
+Set Strict Implicit.
+
+	Inductive java_func :=
+	| pVal (_ : val)
+	| pVarList (_ : list Lang.var) 
+	| pProg (_ : Program)
+	| pCmd (_ : cmd)
+	| pDExpr (_ : dexpr)
+	| pFields (_ : list field)
+	
+	| pMethodSpec
+	| pProgEq
+	| pTriple
+	| pTypeOf
+	| pFieldLookup
+	
+	| pPointsto
+	| pNull
+	
+	| pPlus
+	| pMinus
+	| pTimes
+	| pAnd
+	| pOr
+	| pNot
+	| pLt
+	| pValEq.
+
+	Fixpoint beq_list {A} (f : A -> A -> bool) (xs ys : list A) :=
+		match xs, ys with
+			| nil, nil => true
+			| x::xs, y :: ys => andb (f x y) (beq_list f xs ys)
+			| _, _ => false
+		end.
+
+	Definition typeof_java_func bf :=
+		match bf with
+		    | pVal _ => Some tyVal
+		    | pVarList _ => Some tyVarList
+		    | pProg _ => Some tyProg
+		    | pCmd _ => Some tyCmd
+		    | pDExpr _ => Some tyDExpr
+		    | pFields _ => Some tyFields
+		
+		    | pMethodSpec => Some (tyArr tyString (tyArr tyString (tyArr tyVarList
+		    	 (tyArr tyString (tyArr tySasn (tyArr tySasn tySpec))))))
+		    | pProgEq => Some (tyArr tyProg tySpec)
+		    | pTriple => Some (tyArr tySasn (tyArr tySasn (tyArr tyCmd tySpec)))
+		    
+		    | pTypeOf => Some (tyArr tyString (tyArr tyVal tyProp))
+		    
+		    | pFieldLookup => Some (tyArr tyProg (tyArr tyString (tyArr tyFields tyProp)))
+		    
+		    | pPointsto => Some (tyArr tyVal (tyArr tyString (tyArr tyVal tyAsn)))
+		    
+		    | pNull => Some tyVal
+		    
+		    | pPlus => Some (tyArr tyVal (tyArr tyVal tyVal))
+		    | pMinus => Some (tyArr tyVal (tyArr tyVal tyVal))
+		    | pTimes => Some (tyArr tyVal (tyArr tyVal tyVal))
+		    | pAnd => Some (tyArr tyVal (tyArr tyVal tyVal))
+		    | pOr => Some (tyArr tyVal (tyArr tyVal tyVal))
+		    | pNot => Some (tyArr tyVal tyVal)
+		    | pLt => Some (tyArr tyVal (tyArr tyVal tyVal))
+		    | pValEq => Some (tyArr tyVal (tyArr tyVal tyVal))
+		end.
+
+	Definition java_func_eq (a b : java_func) : option bool :=
+	  match a , b with
+		| pVal a, pVal b => Some (a ?[ eq ] b)
+	    | pVarList a, pVarList b => Some (a ?[ eq ] b)
+	    | pProg a, pProg b => Some (a ?[ eq ] b)
+	    | pCmd a, pCmd b => Some (a ?[ eq ] b)
+	    | pDExpr e1, pDExpr e2 => Some (e1 ?[ eq ] e2)
+	    | pFields a, pFields b => Some (a ?[ eq ] b)
+	        
+	    | pMethodSpec, pMethodSpec => Some true
+	    | pProgEq, pProgEq => Some true
+		| pTriple, pTriple => Some true
+	
+	    | pTypeOf, pTypeOf => Some true
+	
+	    | pPointsto, pPointsto => Some true
+	    | pFieldLookup, pFieldLookup => Some true
+	
+	    | pNull, pNull => Some true
+	    | pPlus, pPlus => Some true
+	    | pMinus, pMinus => Some true
+	    | pTimes, pTimes => Some true
+	    | pAnd, pAnd => Some true
+	    | pOr, pOr => Some true
+	    | pNot, pNot => Some true
+	    | pLt, pLt => Some true
+	    | pValEq, pValEq => Some true
+	    | _, _ => None
+	  end.
+
+    Global Instance RelDec_java_func : RelDec (@eq java_func) := {
+      rel_dec a b := match java_func_eq a b with 
+    	  		       | Some b => b 
+    		 	       | None => false 
+    			     end
+    }.
+
+    Global Instance RelDec_Correct_ilfunc : RelDec_Correct RelDec_java_func.
+    Proof.
+      constructor.
+      destruct x; destruct y; simpl;
+      try solve [ try rewrite Bool.andb_true_iff ;
+                  repeat rewrite rel_dec_correct; intuition congruence ].                  	
+    Qed.
+
+Definition set_fold_fun (x : String.string) (f : field) (P : sasn) :=
+	(`pointsto) (x/V) `f `null ** P.
+
+  	 Definition java_func_symD bf :=
+		match bf as bf return match typeof_java_func bf with
+								| Some t => typD t
+								| None => unit
+							  end with
+              | pProg p => p
+              | pVal v => v
+              | pVarList vs => vs
+              | pCmd c => c
+              | pDExpr e => e
+              | pFields fs => fs
+
+              | pMethodSpec => method_spec
+              | pProgEq => prog_eq
+              | pTriple => triple
+              
+              | pTypeOf => typeof
+                            
+              | pFieldLookup => field_lookup
+              
+              | pPointsto => pointsto
+              
+              | pNull => null
+              
+              | pPlus => eplus
+              | pMinus => eminus
+              | pTimes => etimes
+              | pAnd => eand
+              | pOr => eor
+              | pNot => enot
+              | pLt => elt
+              | pValEq => eeq
+	end.
+
+	Global Instance RSym_JavaFunc : SymI.RSym java_func := {
+	  typeof_sym := typeof_java_func;
+	  symD := java_func_symD;
+	  sym_eqb := java_func_eq
+	}.
+
+	Global Instance RSymOk_JavaFunc : SymI.RSymOk RSym_JavaFunc.
+	Proof.
+		split; intros.
+		destruct a, b; simpl; try apply I; try reflexivity.
+		+ consider (v ?[ eq ] v0); intuition congruence.
+		+ consider (l ?[ eq ] l0); intuition congruence.
+		+ consider (p ?[ eq ] p0); intuition congruence. 
+		+ consider (c ?[ eq ] c0); intuition congruence. 
+		+ consider (d ?[ eq ] d0); intuition congruence. 
+		+ consider (l ?[ eq ] l0); intuition congruence. 
+	Qed.		
+
+
+Definition func := (SymEnv.func + @ilfunc typ + @bilfunc typ + 
+                    @base_func typ + @list_func typ + @open_func typ _ _ + 
+                    @embed_func typ + @later_func typ + java_func)%type.
+
+Section MakeJavaFunc.
+	Definition mkVal v : expr typ func := Inj (inr (pVal v)).
+	Definition mkVarList vs : expr typ func := Inj (inr (pVarList vs)).
+	Definition mkProg P : expr typ func := Inj (inr (pProg P)).
+	Definition mkCmd c : expr typ func := Inj (inr (pCmd c)).
+	Definition mkDExpr e : expr typ func := Inj (inr (pDExpr e)).
+	Definition mkFields fs : expr typ func := Inj (inr (pFields fs)).
+
+	Definition fMethodSpec : expr typ func := Inj (inr pMethodSpec).
+	Definition fProgEq : expr typ func := Inj (inr pProgEq).
+	Definition fTriple : expr typ func := Inj (inr pTriple).
+	Definition fTypeOf : expr typ func := Inj (inr pTypeOf).
+	Definition fFieldLookup : expr typ func := Inj (inr pFieldLookup).
+	Definition fPointsto : expr typ func := Inj (inr pPointsto).
+	Definition mkNull : expr typ func := Inj (inr pNull).
+
+	Definition fPlus : expr typ func := Inj (inr pPlus).
+	Definition fMinus : expr typ func := Inj (inr pMinus).
+	Definition fTimes : expr typ func := Inj (inr pTimes).
+	Definition fAnd : expr typ func := Inj (inr pAnd).
+	Definition fOr : expr typ func := Inj (inr pOr).
+	Definition fNot : expr typ func := Inj (inr pNot).
+	Definition fLt : expr typ func := Inj (inr pLt).
+	Definition fValEq : expr typ func := Inj (inr pValEq).
+
+	Definition mkTriple P c Q : expr typ func := App (App (App fTriple P) Q) c.
+	Definition mkFieldLookup P C f : expr typ func := App (App (App fFieldLookup P) C) f.
+	Definition mkTypeOf C x : expr typ func := App (App fTypeOf C) x.
+	Definition mkProgEq P := App fProgEq P.
+	
+	Definition mkExprList es :=
+		(fold_right (fun (e : dexpr) (acc : expr typ func) => 
+			mkCons tyExpr (mkDExpr e) acc) (mkNil tyExpr) es).
+	
+	Fixpoint evalDExpr (e : dexpr) : expr typ func :=
+		match e with
+			| E_val v => mkConst tyVal (mkVal v)
+			| E_var x => App (fStackGet (func := expr typ func)) (mkString (func := func) x)
+			| E_plus e1 e2 => mkAps fPlus ((evalDExpr e2, tyVal)::(evalDExpr e1, tyVal)::nil) tyVal
+			| E_minus e1 e2 => mkAps fMinus ((evalDExpr e2, tyVal)::(evalDExpr e1, tyVal)::nil) tyVal
+			| E_times e1 e2 => mkAps fTimes ((evalDExpr e2, tyVal)::(evalDExpr e1, tyVal)::nil) tyVal
+			| E_and e1 e2 => mkAps fAnd ((evalDExpr e2, tyVal)::(evalDExpr e1, tyVal)::nil) tyVal
+			| E_or e1 e2 => mkAps fOr ((evalDExpr e2, tyVal)::(evalDExpr e1, tyVal)::nil) tyVal
+			| E_not e => mkAps fNot ((evalDExpr e, tyVal)::nil) tyVal
+			| E_lt e1 e2 => mkAps fLt ((evalDExpr e2, tyVal)::(evalDExpr e1, tyVal)::nil) tyVal
+			| E_eq e1 e2 => mkAps fValEq ((evalDExpr e2, tyVal)::(evalDExpr e1, tyVal)::nil) tyVal
+		end.
+
+
+End MakeJavaFunc.
+
+Require Import Java.Examples.ListModel.
+
+
+Class Environment := { java_env :> @SymEnv.functions typ _}.
+
+Section JavaFunc.
+
+  Context {fs : Environment}.
+
+(* This needs to be parametric. It shouldn't be here 
+Definition fs : @SymEnv.functions typ _ :=
+  SymEnv.from_list
+  	(@SymEnv.F typ _ (tyArr tyVal (tyArr (tyList tyVal) tyAsn)) List::
+  	 @SymEnv.F typ _ (tyArr tyVal (tyArr (tyList tyVal) tyAsn)) NodeList::nil). 
+
+*)
+Check RSym.
+
+  Global Instance RSym_ilfunc : RSym (@ilfunc typ) := 
+	  RSym_ilfunc ilops.
+  Global Instance RSym_bilfunc : RSym (@bilfunc typ) := 
+	  RSym_bilfunc _ bilops.
+  Global Instance RSym_embed_func : RSym (@embed_func typ) :=
+	  RSym_embed_func _ eops.
+  Global Instance RSym_later_func : RSym (@later_func typ) :=
+	  RSym_later_func _ lops.
+
+  Global Instance RSym_open_func : RSym (@open_func typ _ _) :=
+	  @RSym_OpenFunc _ _ _ RType_typ _ _ _ _ _ _ _ _.
+
+  Global Existing Instance RSym_sum.
+  Global Existing Instance RSymOk_sum.
+
+  Global Instance RSym_func : RSym func.
+    repeat (apply RSym_sum; [|apply _]).
+    apply (RSym_func java_env).
+  Defined.
+
+  Global Instance RelDec_expr : RelDec (@eq func) := _.
+
+  Global Instance Expr_expr : ExprI.Expr _ (expr typ func) := @Expr_expr typ func _ _ _.
+  Global Instance Expr_ok : @ExprI.ExprOk typ RType_typ (expr typ func) Expr_expr := ExprOk_expr.
+
+  Require Import MirrorCore.VariablesI.
+  Require Import MirrorCore.Lambda.ExprVariables.
+
+  Global Instance ExprVar_expr : ExprVar (expr typ func) := _.
+  Global Instance ExprVarOk_expr : ExprVarOk ExprVar_expr := _.
+
+  Global Instance ExprUVar_expr : ExprUVar (expr typ func) := _.
+  Global Instance ExprUVarOk_expr : ExprUVarOk ExprUVar_expr := _.
+
+  Definition subst : Type :=
+    FMapSubst.SUBST.raw (expr typ func).
+  Global Instance SS : SubstI.Subst subst (expr typ func) :=
+    @FMapSubst.SUBST.Subst_subst _.
+  Global Instance SU : SubstI.SubstUpdate subst (expr typ func) :=
+    @FMapSubst.SUBST.SubstUpdate_subst _ _. 
+  Global Instance SO : SubstI.SubstOk SS := 
+    @FMapSubst.SUBST.SubstOk_subst typ RType_typ (expr typ func) _ _.
+  Global Instance SUO :SubstI.SubstUpdateOk SU SO :=  @FMapSubst.SUBST.SubstUpdateOk_subst typ RType_typ (expr typ func) _ _ _.
+
+  Global Instance MA : MentionsAny (expr typ func) := {
+    mentionsAny := ExprCore.mentionsAny
+  }.
+
+  Global Instance MAOk : MentionsAnyOk MA _ _.
+  Proof.
+    admit.
+  Qed.
+
+  Lemma evalDexpr_wt (e : dexpr) : 
+	  typeof_expr nil nil (evalDExpr e) = Some tyExpr.
+  Proof.
+    induction e.
+    + simpl; reflexivity.
+    + simpl; reflexivity.
+    + simpl; rewrite IHe1, IHe2; reflexivity.
+    + simpl; rewrite IHe1, IHe2; reflexivity.
+    + simpl; rewrite IHe1, IHe2; reflexivity.
+    + simpl; rewrite IHe1, IHe2; reflexivity.
+    + simpl; rewrite IHe1, IHe2; reflexivity.
+    + simpl; rewrite IHe; reflexivity.
+    + simpl; rewrite IHe1, IHe2; reflexivity.
+    + simpl; rewrite IHe1, IHe2; reflexivity.
+  Qed.
+
+  Definition is_pure (e : expr typ func) : bool :=
+	match e with
+	  | App f P => match embedS f with
+				     | Some (eilf_embed tyPure tySasn) => true
+					 | Some (eilf_embed tyProp tySasn) => true
+					 | _ => false
+				   end
+			
+ 	  | e =>
+ 		match ilogicS e with
+ 		  | Some (ilf_true _) => true
+ 		  | Some (ilf_false _) => true
+ 		  | _ => false
+ 		end
+   end.
+
+  Definition mkPointstoVar x f e : expr typ func :=
+     mkAp tyVal tyAsn 
+          (mkAp tyString (tyArr tyVal tyAsn)
+                (mkAp tyVal (tyArr tyString (tyArr tyVal tyAsn))
+                      (mkConst (tyArr tyVal (tyArr tyString (tyArr tyVal tyAsn))) 
+                               fPointsto)
+                      (App fStackGet (mkString x)))
+                (mkConst tyString (mkString f)))
+          e.
+
+  Definition test_lemma :=
+    @lemmaD typ (expr typ func) RType_typ Expr_expr (expr typ func)
+            (fun tus tvs e => exprD' tus tvs e tyProp)
+            _
+            nil nil.
+End JavaFunc.
