Java/src/Java/Func/Reify.v
@@ -1,0 +1,305 @@
+Require Import MirrorCore.Reify.Reify.
+Require Import MirrorCore.Lambda.Expr.
+
+Require Import Java.Logic.AssertionLogic.
+Require Import Java.Logic.SpecLogic.
+Require Import Java.Language.Program.
+Require Import Java.Language.Lang.
+Require Import Java.Semantics.OperationalSemantics.
+Require Import Java.Func.JavaFunc.
+Require Import Java.Func.JavaType.
+
+Require Import Charge.ModularFunc.ILogicFunc.
+Require Import Charge.ModularFunc.BILogicFunc.
+Require Import Charge.ModularFunc.LaterFunc.
+Require Import Charge.ModularFunc.BaseFunc.
+Require Import Charge.ModularFunc.ListFunc.
+Require Import Charge.ModularFunc.OpenFunc.
+Require Import Charge.ModularFunc.EmbedFunc.
+Require Import Charge.Open.Stack.
+Require Import Charge.Open.Subst.
+Require Import Charge.Open.OpenILogic.
+Require Import Charge.Logics.BILogic.
+Require Import Charge.Logics.Later.
+
+Require Import ExtLib.Structures.Applicative.
+
+Reify Declare Patterns patterns_java_typ := typ.
+
+Reify Declare Patterns patterns_java := (ExprCore.expr typ func).
+
+Local Instance Applicative_Fun A : Applicative (Fun A) :=
+{ pure := fun _ x _ => x
+; ap := fun _ _ f x y => (f y) (x y)
+}.
+
+(*
+Reify Declare Patterns const_for_cmd += ((RHasType cmd ?0) => (fun (c : id cmd) => mkCmd [c] : expr typ func)).
+*)
+
+Require Import MirrorCore.Reify.Reify.
+
+Axiom t : Type.
+Reify Declare Patterns t_pat := t.
+
+
+
+Reify Declare Syntax t_cmd :=
+{ (@Patterns.CPatterns t t_pat) }.
+
+
+Reify Declare Syntax reify_imp_typ :=
+  { 
+  	(@Patterns.CPatterns typ patterns_java_typ)
+  }.
+
+Reify Declare Typed Table term_table : BinNums.positive => reify_imp_typ.
+
+Check term_table.
+
+Locate exprD.
+
+Require Import MirrorCore.ExprI.
+
+Check @exprD.
+Print Expr.
+Print RType.
+Let Ext x := @ExprCore.Inj typ func (inl (inl (inl (inl (inl (inl (inl (inl x)))))))).
+
+Reify Declare Syntax reify_imp :=
+  { (@Patterns.CFirst _
+  		((@Patterns.CVar _ (@ExprCore.Var typ func)) ::
+  	     (@Patterns.CPatterns _ patterns_java) ::
+         (@Patterns.CApp _ (@ExprCore.App typ func)) ::
+    	 (@Patterns.CAbs _ reify_imp_typ (@ExprCore.Abs typ func)) ::
+    	 (@Patterns.CTypedTable _ _ _ term_table Ext) :: nil))
+  }.
+
+Definition stack_get (x : Lang.var) (s : Lang.stack) := s x.
+
+Notation "'ap_eq' '[' x ',' y ']'" :=
+	 (ap (T := Fun Lang.stack) (ap (T := Fun Lang.stack) (pure (T := Fun Lang.stack) (@eq val)) x) y).
+Notation "'ap_pointsto' '[' x ',' f ',' e ']'" := 
+	(ap (T := Fun Lang.stack) (ap (T := Fun Lang.stack) (ap (T := Fun Lang.stack) 
+		(pure (T := Fun Lang.stack) pointsto) (stack_get x)) 
+			(pure (T := Fun Lang.stack) f)) e).
+Notation "'ap_typeof' '[' e ',' C ']'" :=
+	(ap (T := Fun Lang.stack) 
+	    (ap (T := Fun Lang.stack) 
+	        (pure (T := Fun Lang.stack) typeof) 
+	        (pure (T := Fun Lang.stack) C))
+	    e).
+(*
+Definition set_fold_fun (x f : String.string) (P : sasn) :=
+	ap_pointsto [x, f, pure null] ** P.
+*)
+Let _Inj := @ExprCore.Inj typ func.
+
+Require Import Java.Examples.ListModel.
+(*
+Reify Seed Typed Table term_table += 1 => [ (tyArr tyVal (tyArr (tyList tyVal) tyAsn)) , List ].
+Reify Seed Typed Table term_table += 2 => [ (tyArr tyVal (tyArr (tyList tyVal) tyAsn)) , NodeList ].
+*)
+
+Local Notation "x @ y" := (@RApp x y) (only parsing, at level 30).
+Local Notation "'!!' x" := (@RExact _ x) (only parsing, at level 25).
+Local Notation "'?' n" := (@RGet n RIgnore) (only parsing, at level 25).
+Local Notation "'?!' n" := (@RGet n RConst) (only parsing, at level 25).
+Local Notation "'#'" := RIgnore (only parsing, at level 0).
+
+Reify Pattern patterns_java_typ += (@RImpl (?0) (?1)) => (fun (a b : function reify_imp_typ) => tyArr a b).
+
+Reify Pattern patterns_java_typ += (!! asn)  => tyAsn.
+Reify Pattern patterns_java_typ += (!! sasn) => tySasn.
+Reify Pattern patterns_java_typ += (!! (@vlogic Lang.var val)) => tyPure.
+Reify Pattern patterns_java_typ += (!! Prop) => tyProp.
+Reify Pattern patterns_java_typ += (!! spec) => tySpec.
+
+Reify Pattern patterns_java_typ += (!! @prod @ ?0 @ ?1) => (fun (x y : function reify_imp_typ) => tyPair x y).
+Reify Pattern patterns_java_typ += (!! (@list String.string)) => tyVarList.
+Reify Pattern patterns_java_typ += (!! (@list field)) => tyFields.
+Reify Pattern patterns_java_typ += (!! (@list (@Open.expr (Lang.var) val))) => tyVarList.
+Reify Pattern patterns_java_typ += (!! (@list (Lang.var * @Open.expr (Lang.var) val))) => tySubstList.
+Reify Pattern patterns_java_typ += (!! (@substlist Lang.var val)) => tySubstList.
+Reify Pattern patterns_java_typ += (!! @list @ ?0) => (fun x : function reify_imp_typ => tyList x).
+Reify Pattern patterns_java_typ += (!! nat) => tyNat.
+Reify Pattern patterns_java_typ += (!! val) => tyVal.
+Reify Pattern patterns_java_typ += (!! bool) => tyBool.
+Reify Pattern patterns_java_typ += (!! field) => tyString.
+Reify Pattern patterns_java_typ += (!! class) => tyString.
+Reify Pattern patterns_java_typ += (!! @Open.open Lang.var val asn) => tySasn.
+Reify Pattern patterns_java_typ += (!! @Open.open Lang.var val Prop) => tyPure.
+Reify Pattern patterns_java_typ += (!! Lang.var) => tyString.
+Reify Pattern patterns_java_typ += (!! String.string) => tyString.
+Reify Pattern patterns_java_typ += (!! Program) => tyProg.
+Reify Pattern patterns_java_typ += (!! Lang.stack) => tyStack.
+Reify Pattern patterns_java_typ += (!! @Stack.stack Lang.var val) => tyStack.
+Reify Pattern patterns_java_typ += (!! cmd) => tyCmd.
+Reify Pattern patterns_java_typ += (!! dexpr) => tyExpr.
+Reify Pattern patterns_java_typ += (!! (@Open.expr Lang.var val)) => tyExpr.
+Reify Pattern patterns_java_typ += (!! @Subst.subst (String.string) val) => tySubst.
+
+Reify Pattern patterns_java_typ += (!! Fun @ ?0 @ ?1) => (fun (a b : function reify_imp_typ) => tyArr a b).
+
+Reify Pattern patterns_java += (RHasType String.string (?0)) => (fun (s : id String.string) => mkString (func := func) (typ := typ) s).
+Reify Pattern patterns_java += (RHasType field (?0)) => (fun (f : id field) => mkString (func := func) f).
+Reify Pattern patterns_java += (RHasType Lang.var (?0)) => (fun (f : id Lang.var) => mkString (func := func) f).
+Reify Pattern patterns_java += (RHasType val (?0)) => (fun (v : id val) => mkVal v).
+Reify Pattern patterns_java += (RHasType bool (?0)) => (fun (b : id bool) => mkBool (func := func) b).
+Reify Pattern patterns_java += (RHasType nat (?0)) => (fun (n : id nat) => mkNat (func := func) n).
+Reify Pattern patterns_java += (RHasType cmd (?0)) => (fun (c : id cmd) => mkCmd c).
+Reify Pattern patterns_java += (RHasType dexpr (?0)) => (fun (e : id dexpr) => mkDExpr e).
+Reify Pattern patterns_java += (RHasType Program (?0)) => (fun (P : id Program) => mkProg P).
+Reify Pattern patterns_java += (RHasType (list field) (?0)) => (fun (fs : id (list field)) => mkFields fs).
+Reify Pattern patterns_java += (RHasType class (?0)) => (fun (c : id class) => mkString (func := func) c).
+
+Reify Pattern patterns_java += (RHasType (@list dexpr) (?0)) => (fun (es : id (@list dexpr)) => mkExprList es).
+Reify Pattern patterns_java += (RHasType (@list String.string) (?0)) => (fun (vs : id (@list String.string)) => mkVarList vs).
+Reify Pattern patterns_java += (!! (@eq) @ ?0) => (fun (x : function reify_imp_typ) => fEq (func := expr typ func) x).
+
+(** Intuitionistic Operators **)
+Reify Pattern patterns_java += (!! @ILogic.lentails @ ?0 @ #) => (fun (x : function reify_imp_typ) => fEntails (func := expr typ func) x).
+Reify Pattern patterns_java += (!! @ILogic.ltrue @ ?0 @ #) => (fun (x : function reify_imp_typ) => mkTrue (func := func) x).
+Reify Pattern patterns_java += (!! @ILogic.lfalse @ ?0 @ #) => (fun (x : function reify_imp_typ) => mkFalse (func := func) x).
+
+Reify Pattern patterns_java += (!! @ILogic.land @ ?0 @ #) => (fun (x : function reify_imp_typ) => fAnd (func := expr typ func) x).
+Reify Pattern patterns_java += (!! @ILogic.lor @ ?0 @ #) => (fun (x : function reify_imp_typ) => fOr (func := expr typ func) x).
+Reify Pattern patterns_java += (!! @ILogic.limpl @ ?0 @ #) => (fun (x : function reify_imp_typ) => fImpl (func := expr typ func) x).
+
+Reify Pattern patterns_java += (!! @ILogic.lexists @ ?0 @ # @ ?1) => (fun (x y : function reify_imp_typ) => fExists (func := expr typ func) y x).
+
+Reify Pattern patterns_java += (!! @ILogic.lforall @ ?0 @ # @ ?1) => (fun (x y : function reify_imp_typ) => fForall (func := expr typ func) y x).
+(** Embedding Operators **)
+Reify Pattern patterns_java += (!! @ILEmbed.embed @ ?0 @ ?1 @ #) => (fun (x y : function reify_imp_typ) => fEmbed (func := expr typ func) x y).
+
+Reify Pattern patterns_java += (!! @pair @ ?0 @ ?1) => (fun (x y : function reify_imp_typ) => fPair (func := expr typ func) x y).
+
+(** Special cases for Coq's primitives **)
+Reify Pattern patterns_java += (!! True) => (mkTrue (func := func) tyProp).
+Reify Pattern patterns_java += (!! False) => (mkFalse (func := func) tyProp).
+Reify Pattern patterns_java += (!! and) => (fAnd (func := expr typ func) tyProp).
+
+Reify Pattern patterns_java += (!! or) => (fOr (func := expr typ func) tyProp).
+
+Reify Pattern patterns_java += (!! ex @ ?0) => (fun (x : function reify_imp_typ) => fExists (func := expr typ func) x tyProp).
+
+Reify Pattern patterns_java += (RPi (?0) (?1)) => (fun (x : function reify_imp_typ) (y : function reify_imp) =>
+                                                   ExprCore.App (fForall (func := expr typ func) x tyProp) (ExprCore.Abs x y)).
+
+Reify Pattern patterns_java += (RImpl (?0) (?1)) => (fun (x y : function reify_imp) => 
+	ExprCore.App (ExprCore.App (fImpl (func := expr typ func) tyProp) x) y).
+
+(** Separation Logic Operators **)
+Reify Pattern patterns_java += (!! @BILogic.sepSP @ ?0 @ #) => (fun (x : function reify_imp_typ) => (fStar (func := expr typ func) x)).
+Reify Pattern patterns_java += (!! @BILogic.wandSP @ ?0 @ #) => (fun (x : function reify_imp_typ) => (fWand (func := expr typ func) x)).
+Reify Pattern patterns_java += (!! @BILogic.empSP @ ?0 @ #) => (fun (x : function reify_imp_typ) => (mkEmp (func := func) x)).
+
+Reify Pattern patterns_java += (!! @Later.illater @ ?0 @ #) => (fun (x : function reify_imp_typ) => (fLater (func := expr typ func) x)).
+
+Reify Pattern patterns_java += (!! method_spec) => (fMethodSpec).
+
+(** Program Logic **)
+
+
+Reify Pattern patterns_java += (!! triple) => (fTriple).
+Reify Pattern patterns_java += (!! eval @ (RHasType dexpr (?0))) => (fun e : id dexpr => evalDExpr e).
+Reify Pattern patterns_java += (!! stack_get) => (fStackGet (typ := typ) (func := expr typ func)).
+Reify Pattern patterns_java += (!! stack_add (val := val)) => (fStackSet (typ := typ) (func := expr typ func)).
+
+Reify Pattern patterns_java += (!! pointsto) => (fPointsto).
+Reify Pattern patterns_java += (!! prog_eq) => (fProgEq).
+Reify Pattern patterns_java += (!! typeof) => (fTypeOf).
+
+Reify Pattern patterns_java += (!! (@substl_trunc Lang.var val _)) => (fTruncSubst (func := expr typ func) (typ := typ)).
+Reify Pattern patterns_java += (!! (@substl Lang.var val _)) => (fSubst (func := expr typ func) (typ := typ)).
+
+Reify Pattern patterns_java += (!! @nil @ ?0) => (fun (x : function reify_imp_typ) => (fNil (func := expr typ func) x)).
+Reify Pattern patterns_java += (!! @cons @ ?0) => (fun (x : function reify_imp_typ) => (fCons (func := expr typ func) x)).
+Reify Pattern patterns_java += (!! @length @ ?0) => (fun (x : function reify_imp_typ) => (fLength (func := expr typ func) x)).
+Reify Pattern patterns_java += (!! @zip @ ?0 @ ?1) => (fun (x y : function reify_imp_typ) => (fZip (func := expr typ func) x y)).
+Reify Pattern patterns_java += (!! @map @ ?0 @ ?1) => (fun (x y : function reify_imp_typ) => (fMap (func := expr typ func) x y)).
+Reify Pattern patterns_java += (!! @fold_right @ ?0 @ ?1) => (fun (x y : function reify_imp_typ) => (fFold (func := expr typ func) x y)).
+
+Reify Pattern patterns_java += (!! (@apply_subst Lang.var val) @ ?0) => (fun (x : function reify_imp_typ) => fApplySubst (func := expr typ func) x).
+Reify Pattern patterns_java += (!! @subst1 Lang.var val _) => (fSingleSubst (func := expr typ func)).
+Reify Pattern patterns_java += (!! @field_lookup) => (fFieldLookup).
+(** Applicative **)
+Reify Pattern patterns_java += (!! @Applicative.ap @ !! (Fun Lang.stack) @ # @ ?0 @ ?1) => (fun (x y : function reify_imp_typ) => fAp (func := expr typ func) x y).
+Reify Pattern patterns_java += (!! @Applicative.pure @ !! (Fun Lang.stack) @ # @ ?0) => (fun (x : function reify_imp_typ) => fConst (func := expr typ func) x).
+
+Let elem_ctor : forall x : typ, typD x -> @SymEnv.function _ _ :=
+  @SymEnv.F _ _.
+
+Ltac reify_imp e :=
+  let k fs e :=
+      pose e in
+  reify_expr reify_imp k
+             [ (fun (y : @mk_dvar_map _ _ _ _ term_table elem_ctor) => True) ]
+             [ e ].
+
+Require Import ILogic.
+
+Goal (forall (Pr : Program) (C : class) (v : val) (fields : list field), True).
+  intros Pr C v fields.
+  reify_imp (typeof C v).
+
+  reify_imp (field_lookup).
+  reify_imp (field_lookup Pr C fields).
+
+  pose ((fun (_ : @Stack.stack Lang.var val) => null) : @Open.expr Lang.var val) as e2.
+  pose ((fun (_ : Lang.stack) => null) : Lang.stack -> val) as e3.
+
+
+  reify_imp (pure (T := Fun Lang.stack) pointsto).
+
+  reify_imp (fun a b c => pointsto a b c).
+
+  reify_imp e2.
+  
+  reify_imp e3.
+
+  reify_imp (ap (T := Fun Lang.stack) (ap (T := Fun Lang.stack) (pure (@eq val)) e2) e2).
+
+  pose (E_val (vint 3)) as d.
+
+  reify_imp ((ap (ap (T := Fun Lang.stack) (pure (@eq val)) (eval d)) (pure (vbool true)))).
+  
+  generalize String.EmptyString. intro c.
+   reify_imp (ltrue |-- {[ ltrue ]} cread c c c {[ ltrue ]}).
+
+  reify_imp cskip.
+
+  reify_imp (forall P, P /\ P).
+
+  reify_imp (forall x : nat, x = x).
+  reify_imp (exists x : nat, x = x).
+  reify_imp (@map nat nat).
+  reify_imp (@subst1 Lang.var val _).
+  reify_imp (cseq cskip cskip).
+  
+  reify_imp (ILogic.lentails True True).
+
+  reify_imp ((True -> False) -> True).
+  reify_imp (forall P Q, P /\ Q).
+  reify_imp (forall P : sasn, ILogic.lentails ILogic.ltrue P).
+  reify_imp (forall (G : spec) (P Q : sasn), ILogic.lentails G (triple P Q cskip)).
+  generalize (String.EmptyString : String.string).
+  intro x.
+
+  reify_imp stack_get.
+
+  reify_imp (stack_get x).
+
+  reify_imp (x = x).
+
+  reify_imp (@ltrue sasn _).
+  exact I.
+
+Defined.
+
+Ltac reify_aux e n :=
+  let k fs e :=
+      pose e as n in
+  reify_expr reify_imp k
+             [ (fun (y : @mk_dvar_map _ _ _ _ term_table elem_ctor) => True) ]
+             [ e ].
