Java/src/Java/Tactics/Semantics.v
@@ -1,0 +1,172 @@
+Require Import Charge.Logics.ILogic.
+Require Import Charge.Logics.Later.
+Require Import Charge.Logics.ILEmbed.
+Require Import Charge.Open.OpenILogic.
+Require Import Charge.Open.Subst.
+
+Require Import Java.Language.Lang.
+Require Import Java.Language.Program.
+
+Require Import Java.Semantics.OperationalSemantics.
+Require Import Java.Semantics.AxiomaticSemantics.
+
+Require Import Java.Logic.SpecLogic.
+Require Import Java.Logic.AssertionLogic.
+
+Require Import ExtLib.Data.PreFun.
+Require Import ExtLib.Structures.Applicative.
+
+Require Import Java.Func.Reify.
+
+Set Implicit Arguments.
+Set Strict Implicit.
+
+Local Instance Applicative_Fun A : Applicative (Fun A) :=
+{ pure := fun _ x _ => x
+; ap := fun _ _ f x y => (f y) (x y)
+}.
+
+Lemma pull_exists {A} {P : A -> sasn} c Q G
+	(H : forall x, G |-- {[P x]} c {[Q]}) :
+	G |-- {[lexists P]} c {[Q]}.
+Proof.
+  rewrite <- exists_into_precond2.
+  apply lforallR. apply H.
+Qed.
+Print sasn.
+Lemma eq_to_subst x (e : Lang.stack -> val) (P Q : sasn) 
+    (H : apply_subst P (subst1 e x) |-- apply_subst Q (subst1 e x)) :
+	embed (ap_eq [stack_get x, e]) //\\ P |-- Q.
+Proof.
+  
+  admit.
+Qed.
+
+Lemma ent_left_exists {A} (P : sasn) (Q : A -> sasn)
+	(H : exists x, P |-- Q x) :
+	P |-- lexists Q.
+Proof.
+  admit.
+Qed.
+
+Lemma rule_seq c1 c2 (P Q R : sasn) G
+      (Hc1 : G |-- {[P]} c1 {[Q]})
+      (Hc2 : G |-- {[Q]} c2 {[R]}) :
+  G |-- {[P]} cseq c1 c2 {[R]}.
+Proof.
+  apply rule_seq with Q; assumption.
+Qed.
+
+Lemma rule_skip P Q G : P |-- Q -> G |-- {[P]} cskip {[Q]}.
+Proof.
+  intros.
+  eapply roc_post; [eapply rule_skip | apply H].
+Qed.
+	
+Lemma rule_skip2 P G :(* P |-- Q -> *)G |-- {[P]} cskip {[P]}.
+Proof.
+  apply rule_skip. reflexivity.
+Qed.
+
+Lemma rule_if (e : dexpr) c1 c2 (P Q : sasn) G
+      (Hc1 : G |-- {[(@embed (@vlogic Lang.var val) sasn _ 
+                      (ap_eq [eval e, pure (vbool true)])) //\\ P]} c1 {[Q]})
+      (Hc2 : G |-- {[(@embed (@vlogic Lang.var _) sasn _ 
+                      (ap_eq [eval (E_not e), pure (vbool true)])) //\\ P]} c2 {[Q]}) : 
+  G |-- {[P]} cif e c1 c2 {[Q]}. 
+Proof.
+  reify_imp (G |-- {[P]} cif e c1 c2 {[Q]}).
+  eapply rule_if; unfold vlogic_eval, Open.liftn, Open.lift; simpl in *;
+  	[apply Hc1|apply Hc2].
+Qed.
+
+Require Import Charge.Logics.BILogic.
+
+  Lemma rule_read_fwd (x y : Lang.var) (f : field) (e : stack -> val) (P Q : sasn) (G : spec)
+    (HP : P |-- ap_pointsto [y, f, e])
+    (HQ : Exists v : val, (embed (ap_eq [stack_get x, apply_subst e (subst1 (pure (T := Fun stack) v) x)])) //\\
+    					      (apply_subst P (subst1 (pure (T := Fun stack) v) x)) |-- Q) :
+    G |-- {[ P ]} cread x y f {[ Q ]}.
+  Proof.
+    pose proof @rule_read_fwd x y f e P. 
+    unfold Open.liftn, Open.lift, open_eq, stack_get, Open.var_expr in *; simpl in *.
+    rewrite <- HQ , <- H; [apply ltrueR | apply HP].
+  Qed.
+
+
+  Lemma rule_write_fwd (x : Lang.var) (f : field) (e : dexpr) G (P Q F : sasn) (e' : stack -> val)
+        (HP : P |-- ap_pointsto [x, f, e'] ** F) 
+        (HQ : ap_pointsto [x, f, eval e] ** F |-- Q) :
+    G |-- ({[ P ]} cwrite x f e {[ Q ]}).
+  Proof.
+     pose proof @rule_write_frame G P F x f e' e. unfold Open.liftn, Open.lift, open_eq, stack_get, Open.var_expr in *; simpl in *.
+	 rewrite <- HQ, H.
+	 unfold stack. unfold pointsto. unfold eval.
+	 
+	 setoid_rewrite <- sepSPC1 at 2.
+	 reflexivity. 
+	 rewrite HP. 
+	 setoid_rewrite <- sepSPC1 at 2.
+	 reflexivity.
+  Qed.
+
+  Lemma rule_assign_fwd (x : Lang.var) (e : dexpr) G P :
+    G |-- {[ P ]} cassign x e {[ Exists v : val,
+                                 embed (ap_eq [stack_get x, 
+                                               apply_subst (eval e) (subst1 (pure (T := Fun stack) v) x)]) //\\ 
+    							   (apply_subst P (subst1 (pure (T := Fun stack) v) x)) ]}.
+  Proof.
+    pose proof @rule_assign_fwd G P.
+    apply H. reflexivity.
+  Qed.
+
+  Lemma rule_alloc_fwd (x : Lang.var) (C : class) (G : spec) (P Q : sasn) (fields : list field) (Pr : Program) 
+	(Heq : G |-- prog_eq Pr)
+	(Hf : field_lookup Pr C fields) 
+	(Hent : Exists p : val, embed (ap_typeof [stack_get x, C]) //\\
+	                                            embed (ap_eq [stack_get x, pure p]) //\\
+	                                            fold_right (fun f P => ap_pointsto [x, f, pure null] ** P)
+	                                                    (apply_subst P (subst1 (pure (T := Fun stack) p) x)) fields |-- Q) :
+	G |-- {[ P ]} calloc x C {[ Q ]}.
+  Proof.
+  	admit.
+  Qed.
+
+  Lemma rule_static_complete (x : Lang.var) C (m : String.string) (es : list dexpr) (ps : list String.string) (r : Lang.var) G
+    (P Q F Pm Qm : sasn)
+    (HSpec : G |-- |> method_spec C m ps r Pm Qm)
+    (HPre: P |-- apply_subst Pm (substl_trunc (zip ps (@map _ (stack -> val) eval es))) ** F)
+    (HLen: length ps = length es) :
+          G |-- {[ P ]} cscall x C m es {[ Exists v:val, apply_subst Qm (substl_trunc (zip (@cons String.string r ps) 
+                                     (@cons (stack -> val) (stack_get x)
+                                      (@map (stack -> val) _ (fun e => apply_subst e (subst1 (pure (T := Fun stack) v) x)) 
+                                          (@map dexpr (stack -> val) eval es))))) ** 
+                           apply_subst F (subst1 (pure (T := Fun stack) v) x)]}.
+Proof.
+	admit.
+Qed.
+(*
+Lemma rule_dynamic_complete (x y : Lang.var) (m : String.string) (es : list dexpr) (ps : list String.string) C (r : Lang.var) G
+    (P Q F Pm Qm : sasn)
+    (HSpec : G |-- |> method_spec C m ps r Pm Qm)
+    (HPre: P |-- (embed (ap_typeof [stack_get y, C]) //\\ 
+                  apply_subst Pm (substl_trunc (zip ps (@map _ (stack -> val) eval (E_var y :: es))))) ** 
+                 F)
+    (HPost : Exists v:val, embed (ap_typeof [apply_subst (stack_get y) (subst1 (pure (T := Fun stack) v) x), C]) //\\
+                    apply_subst Qm (substl_trunc (zip (@cons String.string r ps) 
+                    (@cons (stack -> val) (stack_get x) (@cons (stack -> val) (apply_subst (stack_get y) (subst1 (pure (T := Fun stack) v) x))
+			        (@map (stack -> val) _ (fun e => apply_subst e (subst1 (pure (T := Fun stack) v) x)) 
+			        (@map dexpr (stack -> val) eval es)))))) ** 
+                    apply_subst F (subst1 (pure (T := Fun stack) v) x) |-- Q)
+    (HLen: length ps = length (E_var y :: es)) :
+           G |-- {[ P ]} cdcall x y m es {[ Q ]}.
+Proof.
+    eapply rule_dcall_forward.
+    eassumption.
+    rewrite HPre. 
+    reflexivity.
+    assumption.
+    rewrite <- HPost.
+    reflexivity.
+Qed.
+*)
