Java/src/Java/Tactics/SymEx.v
@@ -1,0 +1,1200 @@
+Require Import Coq.Strings.String.
+Require Import Coq.PArith.BinPos.
+Require Import ExtLib.Core.RelDec.
+Require Import ExtLib.Data.String.
+Require Import ExtLib.Data.Nat.
+Require Import ExtLib.Data.HList.
+Require Import MirrorCore.Lemma. 
+Require Import MirrorCore.TypesI.
+Require Import MirrorCore.Lambda.Expr.
+Require Import MirrorCore.RTac.RTac.
+Require Import MirrorCore.provers.DefaultProver.
+Require MirrorCore.syms.SymEnv.
+Require MirrorCore.syms.SymSum.
+Require Import MirrorCore.Subst.FMapSubst.
+Require Import MirrorCore.Lambda.ExprLift.
+Require Import MirrorCore.Lambda.ExprSubst.
+Require Import MirrorCore.Lambda.ExprUnify_simul.
+Require Import MirrorCore.Lambda.Red.
+Require Import MirrorCore.Lambda.AppN. 
+Require Import MirrorCore.Lambda.RedAll.
+Require Import MirrorCore.Lambda.ExprVariables.
+Require Import Charge.ModularFunc.ILogicFunc.
+Require Import Charge.Tactics.OrderedCanceller.
+Require Import Charge.Tactics.BILNormalize.
+Require Import Charge.Tactics.SynSepLog.
+Require Import Charge.Tactics.SepLogFold.
+
+Require Import Java.Tactics.Semantics.
+Require Import Java.Func.JavaType.
+Require Import Java.Func.JavaFunc.
+
+Require Import Charge.ModularFunc.BILogicFunc.
+
+Require Import Charge.Tactics.Rtac.ReifyLemma.
+
+Require Import Charge.Tactics.Rtac.PullConjunct.
+
+Require Import MirrorCore.Reify.Reify.
+
+Require Import Java.Func.Reify.
+
+Require Import Charge.Tactics.Rtac.Subst.
+
+
+Require Import Java.Language.Lang.
+Require Import Java.Language.Program.
+ 
+Require Import Charge.Tactics.Rtac.Apply.
+Require Import Charge.Tactics.Rtac.Cancellation.
+Require Import Charge.Tactics.Rtac.Intro.
+Require Import Charge.Tactics.Rtac.EApply.
+Require Import Charge.Tactics.Rtac.Instantiate.
+
+Require Import Coq.Arith.Peano_dec.
+
+Fixpoint mkStars n P Q : expr typ func := 
+	match n with
+		| 0 => mkStar tySasn P Q
+		| S n => mkStar tySasn (mkStars n P Q) (mkStars n P Q)
+	end.
+	
+Definition cancelTest n :=
+      mkForall tySasn tyProp
+      (mkForall tySasn tyProp
+          (mkEntails tySasn (mkStars n (Var 0) (Var 1)) (mkStars n (Var 1) (Var 0)))).
+          
+Section blurb.
+
+Context {fs : Environment}.
+          
+Time Eval vm_compute in typeof_expr nil nil (cancelTest 10).
+Check THEN.
+Check runOnGoals.
+Time Eval vm_compute in 
+	(THEN (REPEAT 10 (INTRO typ func)) 
+	(runOnGoals (CANCELLATION typ func tySasn is_pure))) 
+		nil nil 0 0 (CTop nil nil) (ctx_empty (expr := expr typ func)) (cancelTest 10).
+
+Fixpoint search_NoDup
+    {A} (A_dec: forall a b: A, {a=b}+{a=b->False}) (l: list A) : option (NoDup l) :=
+  match l with
+  | nil => Some (NoDup_nil A)
+  | a::l' =>
+      match search_NoDup A_dec l' with
+      | Some nodup =>
+          match In_dec A_dec a l' with
+          | left isin => None
+          | right notin => 
+ 			match search_NoDup A_dec l' with
+ 				| Some pf => Some (NoDup_cons _ notin pf)
+ 				| None => None         
+            end
+          end
+      | None => None
+      end
+  end.
+(*
+
+
+Definition list_notin_set lst s :=
+  	fold_right (fun a acc => andb (SS.for_all (fun b => negb (string_dec a b)) s) acc) true lst.
+
+Definition method_specI : stac typ (expr typ func) subst :=
+  fun tus tvs s lst e =>
+    match e with
+    	| mkEntails [l, mkProgEq [mkProg [P]], mkMethodSpec [C, m, mkVarList [args], mkString [r], p, q]] => 
+    	      match C, m with
+    	        | Inj (inl (inr (pString Cname))), Inj (inl (inr (pString Mname))) => 
+    	          match SM.find Cname (p_classes P) with
+    	          	| Some Class => 
+    	          	  match SM.find Mname (c_methods Class) with
+    	          	    | Some Method => 
+						  match search_NoDup Coq.Strings.String.string_dec args with
+						  	| Some pf => 
+						  	  match eq_nat_dec (length args) (length (m_params Method)) with
+						  	    | left pf' => 
+						  	      if list_notin_set args (modifies (m_body Method)) then
+						  	        More tus tvs s lst 
+						  	        mkEntails [l, mkProgEq [mkProg [P]], 
+						  	                      mkTriple [mkApplyTruncSubst [tyAsn, p, mkSubstList [mkVarList [args], mkExprList [map E_var (m_params Method)]] ], mkCmd [m_body Method], 
+						  	                               mkApplyTruncSubst [tyAsn, q, mkSubstList [mkVarList [r::args], mkConsExprList [App fEval (mkExpr [m_ret Method]), mkExprList[map E_var (m_params Method)]]] ]]]
+						  	      else
+						  	        @Fail _ _ _
+						  	    | right _ => @Fail _ _ _
+						  	  end 
+						  	| None => @Fail _ _ _
+						  end
+    	          	    | None => @Fail _ _ _
+    	          	  end
+    	          	| None => @Fail _ _ _
+    	          end
+    	        | _, _ => @Fail _ _ _
+    	      end
+      	| _ => @Fail _ _ _
+    end.
+*)
+
+(** Skip **)
+Definition skip_lemma : lemma typ (expr typ func) (expr typ func).
+reify_lemma reify_imp rule_skip.
+Defined.
+Print skip_lemma.
+
+Lemma skip_lemma_sound : 
+	lemmaD (exprD'_typ0 (T:=Prop)) nil nil skip_lemma.
+Proof.
+  unfold lemmaD; simpl; intros.
+  unfold exprT_App, exprT_Inj, Rcast_val, Rcast in * ; simpl in *.
+  apply rule_skip. apply H.
+Qed.
+
+Example test_skip_lemma : test_lemma skip_lemma. Admitted.
+
+Definition skip_lemma2 : lemma typ (expr typ func) (expr typ func).
+reify_lemma reify_imp rule_skip2.
+Defined.
+Print skip_lemma2.
+
+Example test_skip_lemma2 : test_lemma skip_lemma2. Admitted.
+
+Definition seq_lemma (c1 c2 : cmd) : lemma typ (expr typ func) (expr typ func).
+Proof.
+  reify_lemma reify_imp (@rule_seq c1 c2).
+Defined.
+Print seq_lemma.
+
+Lemma seq_lemma_sound c1 c2 : 
+	lemmaD (exprD'_typ0 (T:=Prop)) nil nil (seq_lemma c1 c2).
+Proof.
+  unfold lemmaD; simpl; intros.
+  unfold exprT_App, exprT_Inj, Rcast_val, Rcast in * ; simpl in *.
+  eapply rule_seq; [apply H | apply H0].
+Qed.
+
+Example test_seq_lemma (c1 c2 : cmd) : test_lemma (seq_lemma c1 c2). Admitted.
+
+Definition if_lemma (e : dexpr) (c1 c2 : cmd) : lemma typ (expr typ func) (expr typ func).
+Proof.
+  reify_lemma reify_imp (@rule_if e c1 c2).
+Defined.
+
+Require Import ExtLib.Tactics.
+(*
+Lemma if_lemma_sound e c1 c2 : 
+	lemmaD (exprD'_typ0 (T:=Prop)) nil nil (if_lemma e c1 c2).
+Proof.
+  remember (exprD nil nil (evalDExpr e) tyExpr).
+  Check rule_if.
+  unfold lemmaD; simpl.
+  unfold lemmaD', exprD'_typ0.
+  unfold le
+  unfold if_lemma.
+  destruct o.
+  unfold exprD in Heqo. simpl in Heqo.
+  remember (ExprDsimul.ExprDenote.exprD' nil nil tyVal (evalDExpr e)).
+  destruct o; inv_all; subst; try congruence.
+  unfold lemmaD, lemmaD', exprD'_typ0, ExprDsimul.ExprDenote.exprD'; simpl in *; intros.
+ unfold ExprDsimul.ExprDenote.exprD' in *; simpl in *; intros.
+ unfold exprT_App, exprT_Inj, Rcast_val, Rcast in *; simpl in *.
+ unfold OpenFunc.typ2_cast_bin, OpenFunc.typ3_cast_bin in *; simpl in *.
+ unfold exprT, OpenT in *; simpl in *.
+ rewrite <- Heqo0.
+ unfold ExprDsimul.ExprDenote.exprD' in Heqo0. simpl in Heqo0.
+ rewrite <- Heqo0.
+ repeat red.
+ setoid_rewrite <- Heqo.
+ rewrite <- Heqo.
+    unfold exprT_App, exprT_Inj, Rcast_val, Rcast in * ; simpl in *.
+    eapply rule_if; [eapply H | eapply H0].
+  + unfold lemmaD; simpl; intros.
+    unfold exprT_App, exprT_Inj, Rcast_val, Rcast in * ; simpl in *.
+    eapply rule_if; [eapply H | eapply H0].
+  + unfold lemmaD; simpl; intros.
+    unfold exprT_App, exprT_Inj, Rcast_val, Rcast in * ; simpl in *.
+    eapply rule_if; [eapply H | eapply H0].
+
+  Print if_lemma.
+  vm_compute.
+  unfold lemmaD'. simpl.
+  unfold exprD'_typ0. simpl.
+  unfold ExprDsimul.ExprDenote.exprD'.
+  simpl.
+  unfold if_lemma. simpl.
+  apply rule_skip. apply H.
+Qed.
+*)
+Example test_if_lemma e (c1 c2 : cmd) : test_lemma (if_lemma e c1 c2). Admitted.
+
+Definition read_lemma (x y : var) (f : field) : lemma typ (expr typ func) (expr typ func).
+Proof.  
+  reify_lemma reify_imp (@rule_read_fwd x y f).
+Defined.
+
+Lemma read_lemma_sound x y f : 
+	lemmaD (exprD'_typ0 (T:=Prop)) nil nil (read_lemma x y f).
+Proof.
+  (*
+  unfold lemmaD; simpl; intros.
+  unfold exprT_App, exprT_Inj, Rcast_val, Rcast, OpenFunc.typ3_cast_bin, OpenFunc.typ2_cast_bin, eq_rect_r in * ; simpl in *.
+  eapply rule_read_fwd; [eapply H | eapply H0].
+  *)
+  admit.
+Qed.
+
+
+Example test_read_lemma x y f : test_lemma (read_lemma x y f). Admitted.
+
+Set Printing Width 140.
+
+Definition write_lemma (x : var) (f : field) (e : dexpr) : lemma typ (expr typ func) (expr typ func).
+Proof.
+  reify_lemma reify_imp (@rule_write_fwd x f e).
+Defined.
+(*
+Lemma write_lemma_sound x f e : 
+	lemmaD (exprD'_typ0 (T:=Prop)) nil nil (write_lemma x f e).
+Proof.
+  induction e.
+  Check evalDExpr.
+  unfold lemmaD, lemmaD'; simpl; intros.
+  unfold exprT_App, exprT_Inj, Rcast_val, Rcast, OpenFunc.typ3_cast_bin, OpenFunc.typ2_cast_bin, eq_rect_r, 
+  fPointsto, typ2_cast_bin, BaseFunc.mkString; simpl.
+  unfold exprD'_typ0; simpl.
+  unfold ExprDsimul.ExprDenote.exprD'; simpl.
+  vm_compute.
+  eapply rule_write_fwd; [eapply H | eapply H0].
+Qed.
+*)
+
+Example test_write_lemma x f e : test_lemma (write_lemma x f e). Admitted.
+
+Definition assign_lemma (x : var) (e : dexpr) : lemma typ (expr typ func) (expr typ func).
+Proof.
+  reify_lemma reify_imp (@rule_assign_fwd x e).
+Defined.
+Print assign_lemma.
+Example test_assign_lemma x e : test_lemma (assign_lemma x e). Admitted.
+
+Definition alloc_lemma (x : var) (C : class) : lemma typ (expr typ func) (expr typ func).
+Proof.
+  reify_lemma reify_imp (@rule_alloc_fwd x C).
+Defined.
+Example test_alloc_lemma x C : test_lemma (alloc_lemma x C). Admitted.
+
+Definition pull_exists_lemma : lemma typ (expr typ func) (expr typ func).
+Proof.
+  reify_lemma reify_imp (@pull_exists val).
+Defined.
+Example test_pull_exists_lemma : test_lemma pull_exists_lemma. Admitted.
+Eval vm_compute in pull_exists_lemma.
+
+Definition ent_exists_right_lemma : lemma typ (expr typ func) (expr typ func).
+Proof.
+  reify_lemma reify_imp (@ent_left_exists val).
+Defined.
+Example test_pull_exists_lemma2 : test_lemma ent_exists_right_lemma. Admitted.
+
+Definition eq_to_subst_lemma : lemma typ (expr typ func) (expr typ func).
+Proof.
+  reify_lemma reify_imp eq_to_subst.
+Defined.
+Eval vm_compute in eq_to_subst_lemma.
+Example test_eq_lemma : test_lemma (eq_to_subst_lemma). Admitted.
+Check rule_static_complete.
+Definition scall_lemma (x : Lang.var) (C : class) (m : string) (es : list dexpr) 
+  : lemma typ (expr typ func) (expr typ func).
+Proof.
+  reify_lemma reify_imp rule_static_complete.
+Qed.
+
+Print scall_lemma.
+
+Print pull_exists_lemma.
+
+Example test_pull_exists : test_lemma (pull_exists_lemma). Admitted.
+
+Require Import Charge.ModularFunc.BaseFunc.
+
+Definition fieldLookupTac : rtac typ (expr typ func) :=
+	fun tus tvs n m c s e =>
+		match e with
+		  | App (App (App (Inj (inr pFieldLookup)) (Inj (inr (pProg P)))) C) f =>
+		    match baseS C with
+		      | Some C' =>
+		        match C' with
+		          | pString C'' =>
+				  	match class_lookup C'' P with
+		    	      | Some Class =>
+		    	        match @exprUnify (ctx_subst c) typ func _ _ _ _ _ 3
+		                                 tus tvs 0 f (mkFields (c_fields Class)) tyVarList s with
+		                  | Some s => Solved s
+		                  | None   => Fail
+		                end
+		    	      | None => Fail 
+				    end
+				  | _ => Fail
+				end
+			  | None => Fail
+			end
+		  | _ => Fail
+		end.
+
+Definition FIELD_LOOKUP := fieldLookupTac.
+
+Require Import ExtLib.Tactics.
+
+
+Lemma FIELD_LOOKUP_sound : rtac_sound FIELD_LOOKUP.
+Proof.
+  unfold rtac_sound, rtac_spec; intros.
+  unfold FIELD_LOOKUP, fieldLookupTac in H.
+  destruct g; subst; try apply I.
+  forward.
+  simpl in H10.
+  forward.
+  SearchAbout exprUnify'.
+  Print exprUnify'.
+  Print ExprUnify_common.unify_sound_ind.
+  pose proof (exprUnify_sound).
+  specialize(H13 (ctx_subst ctx) typ func _ _ _ _ _ _ _ _ _ _ 3).
+  red in H13.
+  red in H13.
+  apply H13 with (tv' := nil) in H10; clear H13; [|assumption].
+  forward_reason; split; auto.
+  forward. simpl in H13.
+  simpl in H15.
+  unfold Ctx.propD, exprD'_typ0 in H15.
+  forward; inv_all; subst.
+  simpl in H15.
+  autorewrite with exprD_rw in H15; [|apply _];
+  simpl in H15; forward; inv_all; subst.
+  autorewrite with exprD_rw in H0.
+  simpl in H0; forward; inv_all; subst.
+  autorewrite with exprD_rw in H2; [|apply _];
+  simpl in H2; forward; inv_all; subst.
+  autorewrite with exprD_rw in H2; [|apply _];
+  simpl in H2; forward; inv_all; subst.
+  unfold funcAs in H2. simpl in H2.
+  forward; inv_all; subst.
+  pose proof (pctxD_substD H12 H14).
+  destruct H as [? [? ?]].
+  specialize (H13 _ _ _ H5 eq_refl H).
+  forward; inv_all; subst.
+  destruct H6 as [? [? ?]].
+  pose proof (substD_pctxD _ H10 H14 H6).
+  destruct H13 as [? [? ?]].
+  simpl in *. unfold Expr_expr.
+  rewrite H13.
+  split. admit.
+  intros. unfold exprT_App, exprT_Inj in *; simpl in *.
+  destruct e0; inv_all; try congruence.
+  destruct f; try congruence.
+  destruct s1; try congruence.
+  destruct s1; try congruence.
+  destruct s1; try congruence.
+  destruct s1; try congruence.
+  destruct s1; try congruence.
+  inv_all; subst. simpl in *.
+  Check Ap_pctxD.
+  gather_facts.
+  eapply Pure_pctxD; eauto.
+  intros.
+  specialize (H7 _ _ H8).
+  destruct H7 as [? ?]. specialize (H15 HList.Hnil). simpl in H15.
+  rewrite H15; clear H15.
+  unfold field_lookup. exists c; split; [|reflexivity].
+  autorewrite with exprD_rw in H3; [|apply _];
+  simpl in H2; forward; inv_all; subst.
+  simpl.
+  unfold eq_rect_r. simpl.
+  
+  Require Import ExtLib.Data.String.
+  
+  Lemma class_lookup_sound s p c (H : class_lookup s p = Some c) : In (s, c) (p_classes p).
+  Proof.
+    destruct p. induction p_classes; simpl in *.
+    * unfold class_lookup in H. simpl in H; congruence.
+    * unfold class_lookup in H. simpl in H.
+      destruct a; simpl in *. consider (s ?[ eq ] s0); intros; subst.
+      + left. rewrite rel_dec_eq_true in H; inv_all; subst; [reflexivity| apply _|reflexivity].
+      + right. rewrite rel_dec_neq_false in H; [apply IHp_classes; apply H | apply _ | apply H0].
+  Qed.
+  
+  apply class_lookup_sound.
+  apply H9.
+  apply _.
+Qed.
+
+Require Import Charge.ModularFunc.ListFunc.
+
+	Definition foldTac (e : expr typ func) (args : list (expr typ func))
+	: expr typ func :=
+	  match listS e with
+	    | Some (pFold t u) =>
+	      match args with
+	        | f :: acc :: (Inj (inr (pFields fs)))::nil =>
+	            fold_right (fun x acc => beta (beta (App (App f (mkString x)) acc))) acc fs
+	        | _ => apps e args
+	      end
+	    | _ => apps e args
+	  end.
+
+Require Import MirrorCore.Lambda.ExprTac.
+
+  Lemma foldTacOk : partial_reducer_ok foldTac.
+  Proof.
+    unfold partial_reducer_ok; intros.
+    unfold foldTac.
+    remember (listS e); destruct o; [| exists val; tauto].
+    destruct l; try (exists val; tauto).
+    destruct es; try (exists val; tauto).
+    destruct es; try (exists val; tauto).
+    destruct es; try (exists val; tauto).
+    destruct e2; try (exists val; tauto).
+    destruct f; try (exists val; tauto).
+    
+    destruct j; try (exists val; tauto).
+    destruct es; try (exists val; tauto).
+    destruct e; simpl in Heqo; try congruence.
+    destruct f; simpl in Heqo; try congruence.
+    destruct s; simpl in Heqo; try congruence.
+    destruct s; simpl in Heqo; try congruence.
+    destruct s; simpl in Heqo; try congruence.
+    destruct s; simpl in Heqo; try congruence.
+    inv_all; subst.
+    autorewrite with exprD_rw in H; simpl in H; forward; inv_all; subst.
+    autorewrite with exprD_rw in H; simpl in H; forward; inv_all; subst; [|apply _].
+    autorewrite with exprD_rw in H; simpl in H; forward; inv_all; subst; [|apply _].
+    autorewrite with exprD_rw in H0; simpl in H0; forward; inv_all; subst; [|apply _].
+    autorewrite with exprD_rw in H2; simpl in H2; forward; inv_all; subst; [|apply _].
+    unfold funcAs in H2. 
+    Opaque type_cast.
+    simpl in H2. forward; inv_all; subst. red in r. inv_all.
+    inversion r; subst.
+    rewrite (UIP_refl r) in H4. unfold Rcast in H4; simpl in H4.
+    inversion H4; unfold eq_rect_r in H6; simpl in H6.
+    subst. clear H4.
+    clear H2 r.
+    Opaque beta.
+    simpl.
+    unfold exprT_App, eq_rect_r. simpl.
+    cut (exists val' : exprT tus tvs (typD t),
+  ExprDsimul.ExprDenote.exprD' tus tvs t
+    (fold_right
+       (fun (x : string) (acc : expr typ func) =>
+        beta (beta (App (App e0 (mkString x)) acc))) e1 l) = Some val' /\
+  (forall (us : hlist typD tus) (vs : hlist typD tvs),
+   fold_right (e4 us vs) (e3 us vs) (exprT_Inj tus tvs l us vs) = val' us vs)).
+   intros [? [? ?]].
+   eexists; split; [eassumption | intros; apply H4].
+    induction l; simpl; intros.
+
+    + exists e3; tauto.
+    + destruct IHl as [? [? ?]].
+      eexists; split; [|intros; reflexivity].
+
+  Lemma exprD'_remove_beta tus tvs t e de (H : exprD' tus tvs e t = Some de) :
+    exprD' tus tvs (beta e) t = Some de.
+  Proof.
+    pose proof (beta_sound tus tvs e t).
+    unfold exprD' in *. simpl in *. forward; inv_all; subst.
+	Require Import FunctionalExtensionality.
+	f_equal. symmetry.
+    apply functional_extensionality; intros.
+    apply functional_extensionality; intros.
+    apply H2.
+  Qed.
+  
+  
+      do 2 (apply exprD'_remove_beta).
+      unfold exprD'. simpl.
+      
+      red_exprD; [|apply _].
+      pose proof (exprD_typeof_Some).
+      specialize (H5  _ _ _ _ _ _ _ _ _ _ _ _ _ H2). rewrite H5; clear H5.
+      red_exprD; [|apply _].
+      forward; inv_all; subst.
+      unfold mkString. forward.
+      red_exprD; [|apply _]. 
+      Transparent type_cast.
+      unfold funcAs. simpl.
+	  f_equal. unfold exprT_App; simpl. 
+	  unfold eq_rect_r. simpl.
+	  apply functional_extensionality; intros.
+	  apply functional_extensionality; intros.
+	  rewrite H4. reflexivity.
+Qed.
+SearchAbout partial_reducer_ok.
+
+Print partial_reducer_ok.
+Print apps_reducer.
+Print full_reducer_ok.
+Print full_reducer.
+Check @idred.
+SearchAbout idred.
+Print idred.
+Print idred'.
+Check @beta_all.
+
+Definition FOLD := SIMPLIFY (typ := typ) (fun _ _ _ _ => (beta_all (fun _ => foldTac))).
+
+Require Import ExtLib.Tactics.Consider.
+Require Import ExtLib.Tactics.
+Require Import MirrorCore.Lambda.RedAll.
+Print partial_reducer.
+
+(*
+  Lemma foldTacOk2 : partial_reducer_ok foldTac.
+  Proof.
+    unfold full_reducer_ok; intros.
+    Print var_termsP.
+    Print partial_reducer_ok.
+    unfold exprT, OpenT in P.
+    unfold foldTac.
+    remember (listS e). destruct o.
+    Focus 2.
+    simpl.
+  Qed.
+*)
+Lemma FOLD_sound : rtac_sound FOLD.
+Proof.
+  admit.
+  (*
+  unfold FOLD.
+  apply SIMPLIFY_sound.
+  intros; simpl.
+  forward.
+  rewrite <- H.
+  simpl.
+  unfold Ctx.propD, exprD'_typ0 in H3; forward; inv_all; subst.
+  destruct (beta_all_sound foldTacOk _ _ e0 H3) as [v [H4 H5]].
+  apply beta_all_sound.
+  Check beta_all_sound.
+  (* beta_all_sound is missing *)
+  
+  *)
+Qed.
+Check apps.
+Definition BETA := SIMPLIFY (typ := typ) (fun _ _ _ _ => beta_all (fun _ => @apps typ func)).
+
+Lemma BETA_sound : rtac_sound BETA.
+Proof.
+  unfold BETA.
+  apply SIMPLIFY_sound.
+  intros; simpl; forward.
+  (*
+  SearchAbout full_reducer.
+  assert (full_reducer_ok (fun _ => apps (sym := func))). {
+    clear.
+    intros e vars tus tvs tus' tvs' P Hvars es t targs Hexpr.
+  }
+  unfold full_reducer_ok.
+  
+  Print full_reducer.
+  pose proof (beta_all_sound).
+  SearchAbout beta_all.
+  rewrite <- H.*)
+  admit.
+Qed.
+
+Definition THEN' := @MirrorCore.RTac.Then.THEN typ (expr typ func).
+Require Import Charge.Tactics.Rtac.Minify.
+
+Let EAPPLY lem := THEN' (EAPPLY typ func lem) (MINIFY typ func).
+
+Definition THEN (r1 r2 : rtac typ (expr typ func)) := 
+  THEN (THEN (THEN (INSTANTIATE typ func) (runOnGoals r1)) (runOnGoals (INSTANTIATE typ func))) (runOnGoals r2).
+
+Definition EQSUBST := THEN (EAPPLY eq_to_subst_lemma) (SUBST typ func).
+
+
+
+(*
+Notation "'ap_eq' '[' x ',' y ']'" :=
+	 (ap (T := Fun stack) (ap (T := Fun stack) (pure (T := Fun stack) (@eq val)) x) y).
+*)
+
+Require Import Charge.ModularFunc.OpenFunc.
+Require Import Charge.ModularFunc.BaseFunc.
+Require Import Charge.ModularFunc.EmbedFunc.
+
+Definition match_ap_eq (e : expr typ func) : bool :=
+	match e with 
+	  | App emb (App (App f (App (App g (App h e)) x)) y) =>
+	  	match embedS emb, open_funcS f, open_funcS g, open_funcS h, baseS e with
+	  		| Some (eilf_embed _ _), Some (of_ap _ _), Some (of_ap _ _), Some (of_const _), Some (pEq _) => true
+	  		| _, _, _, _, _ => false
+	  	end
+	  | _ => false
+	end.
+
+Definition PULLEQL := PULLCONJUNCTL typ func match_ap_eq ilops.
+
+                        (*
+	THEN (INSTANTIATE typ func subst) (runOnGoals (THEN (THEN (TRY FIELD_LOOKUP) 
+		(runOnGoals (CANCELLATION typ func subst tySpec (fun _ => false)))) (runOnGoals FOLD))) ::
+		solve_entailment :: nil).
+	           *)
+Require Import Charge.SetoidRewrite.AutoSetoidRewrite.
+Require Import Charge.SetoidRewrite.Base.
+Require Import Charge.SetoidRewrite.ILSetoidRewrite.
+Require Import Charge.SetoidRewrite.BILSetoidRewrite.
+
+  Definition spec_respects (e : expr typ func) (_ : list (RG (expr typ func)))
+	   (rg : RG (expr typ func)) : m (expr typ func) :=
+	   match e with
+	     | Inj (inr pTriple) =>
+	       rg_bind (unifyRG (@rel_dec (expr typ func) _ _) rg
+	         (RGrespects (RGflip (RGinj (fEntails tySasn)))
+	           (RGrespects (RGinj (fEq tyCmd))
+	             (RGrespects (RGinj (fEntails tySasn))
+	               (RGinj (fEntails tySpec))))))
+	         (fun _ => rg_ret fTriple)
+	     | _ => rg_fail
+	   end.
+
+Definition step_unfold vars rw :=
+  setoid_rewrite vars _ (fEntails : typ -> expr typ func) rw
+    (sr_combine il_respects
+               (sr_combine (@il_respects_reflexive typ func _ _ _ ilops _ _)
+                                        (sr_combine bil_respects
+                                                    (sr_combine eq_respects 
+                                                    (sr_combine spec_respects refl)))))
+    (fun _ => rw_fail).
+    
+  Definition STEP_REWRITE rw : rtac typ (expr typ func) :=
+    fun tus tvs lus lvs c s e =>
+      match step_unfold (getVars c) rw tyProp e with
+        | Some (e', _) => More s (GGoal e')
+        | _ => More s (GGoal e)
+      end.
+
+Definition PULL_TRIPLE_EXISTS : rtac typ (expr typ func) :=
+  THEN (THEN (EAPPLY pull_exists_lemma) (INTRO typ func)) BETA.
+
+Definition solve_entailment (rw : rewriter (typ := typ) (func := func)) : rtac typ (expr typ func) :=
+	THEN (INSTANTIATE typ func) 
+		(FIRST (SOLVE (CANCELLATION typ func tySasn is_pure) ::
+	           (THEN (THEN (THEN (THEN PULLEQL (REPEAT 1000 EQSUBST)) 
+	           (STEP_REWRITE rw)) (REPEAT 1000 (INTRO typ func))) 
+	              (CANCELLATION typ func tySasn is_pure)::
+	           nil))).
+
+Definition solve_alloc rw : rtac typ (expr typ func) :=
+    THEN (INSTANTIATE typ func)
+    (FIRST (SOLVE (CANCELLATION typ func tySpec (fun _ => false)) ::
+                        FIELD_LOOKUP ::
+                        THEN FOLD (solve_entailment rw) :: nil)).
+
+Check MINIFY.
+Print rtacK.
+Check runOnGoals (SUBST typ func).
+Check THENK.
+Print rtacK.
+
+Definition simStep (rw : rewriter (typ := typ) (func := func)) (r : rtac typ (expr typ func)) :=
+    THEN (THEN (THEN (THEN (SUBST typ func)
+    	(TRY PULL_TRIPLE_EXISTS)) (STEP_REWRITE rw)) (REPEAT 10 PULL_TRIPLE_EXISTS)) r.
+
+Fixpoint tripleE (c : cmd) rw : rtac typ (expr typ func) :=
+	match c with
+	    | cskip => simStep rw (THEN (EAPPLY skip_lemma) (solve_entailment rw))
+	    | calloc x C => simStep rw (THEN (EAPPLY (alloc_lemma x C)) 
+	        (FIRST (solve_alloc rw::solve_entailment rw::nil)))
+		| cseq c1 c2 => simStep rw (THEN' (EAPPLY (seq_lemma c1 c2))
+		    (THENK (runOnGoals (TRY (tripleE c1 rw))) (THENK (MINIFY typ func) (runOnGoals (tripleE c2 rw)))))
+		| cassign x e => simStep rw (THEN (EAPPLY (assign_lemma x e)) (solve_entailment rw))
+		| cread x y f => simStep rw (THEN (EAPPLY (read_lemma x y f)) (solve_entailment rw))
+		| cif e c1 c2 => simStep rw (THEN (EAPPLY (if_lemma e c1 c2)) (solve_entailment rw))
+		| cwrite x f e => simStep rw (THEN (EAPPLY (write_lemma x f e)) (solve_entailment rw))
+		| _ => IDTAC
+	end.
+
+Definition symE rw : rtac typ (expr typ func) :=
+	(fun tus tvs n m ctx s e => 
+		(match e return rtac typ (expr typ func) with 
+			| App (App (Inj f) G) H =>
+			  match ilogicS f, H with
+			  	| Some (ilf_entails tySpec), (* tySpec is a pattern, should be checked for equality with tySpec *)
+			  	  App (App (App (Inj (inr pTriple)) P) Q) (Inj (inr (pCmd c))) =>
+			  	  	tripleE c rw
+			  	| _, _ => FAIL
+			  end
+			| _ => FAIL
+		end) tus tvs n m ctx s e).  
+
+Definition runTac rw := 
+   (THEN (THEN (REPEAT 1000 (INTRO typ func)) (symE rw)) 
+	(INSTANTIATE typ func)).
+	
+Lemma runTac_sound rw : rtac_sound (runTac rw).
+Proof.
+  admit.
+Qed.
+
+Definition mkPointsto (x : expr typ func) (f : field) (e : expr typ func) : expr typ func :=
+   mkAp tyVal tyAsn 
+        (mkAp tyString (tyArr tyVal tyAsn)
+              (mkAp tyVal (tyArr tyString (tyArr tyVal tyAsn))
+                    (mkConst (tyArr tyVal (tyArr tyString (tyArr tyVal tyAsn))) 
+                             fPointsto)
+                    x)
+              (mkConst tyString (mkString f)))
+        e.
+        
+Require Import Java.Semantics.OperationalSemantics.
+Require Import Java.Logic.SpecLogic.
+Require Import Java.Logic.AssertionLogic.
+Require Import Java.Examples.ListClass.
+Require Import Charge.Logics.ILogic.
+
+Fixpoint seq_skip n := 
+	match n with
+	  | 0 => cskip
+	  | S n => cseq cskip (seq_skip n)
+	end.
+
+Require Import ExtLib.Structures.Applicative.
+Local Instance Applicative_Fun A : Applicative (Fun A) :=
+{ pure := fun _ x _ => x
+; ap := fun _ _ f x y => (f y) (x y)
+}.
+
+Definition testSkip n : Prop :=
+  forall (G : spec) (P : sasn), G |-- triple P P (seq_skip n).
+
+Lemma INTRO_sound : rtac_sound (INTRO typ func).
+Proof.
+  admit.
+Qed.
+
+Require Import Java.Tactics.Tactics.
+Check IDTAC_sound.
+
+Ltac rtac_result reify term_table tac :=
+	  let name := fresh "e" in
+	  match goal with
+	    | |- ?P => 
+	      reify_aux reify term_table P name;
+	      let t := eval vm_compute in (typeof_expr nil nil name) in
+	      let goal := eval unfold name in name in 
+	      match t with
+	        | Some ?t =>
+	          let goal_result := constr:(run_tac tac (GGoal name)) in 
+	          let result := eval vm_compute in goal_result in 
+	          idtac result
+	        | None => idtac "expression " goal "is ill typed" t 
+	      end
+	  end.
+	  
+Lemma test_skip_lemma3 : testSkip 10.
+Proof.
+  idtac "start".
+  unfold testSkip; simpl.
+  
+  Time run_rtac reify_imp term_table (@runTac_sound rw_fail).
+Time Qed.
+
+Definition test_alloc : expr typ func :=
+	mkEntails tySpec (mkProgEq (mkProg ListProg))
+		(mkTriple (mkTrue tySasn) (mkCmd (cseq (calloc "x" "NodeC") cskip)) (mkFalse tySasn)).
+
+Require Import Charge.Logics.BILogic.
+  
+  Lemma test_alloc_correct : 
+  prog_eq ListProg |-- triple empSP lfalse ((calloc "x" "NodeC");;Skip).
+Proof.
+  Time run_rtac reify_imp term_table (@runTac_sound rw_fail).
+  unfold open_func_symD. simpl.
+  admit.
+Qed.
+
+Lemma test_read : ltrue |-- 
+    triple 
+      (ap_pointsto [("o": var), ("f" : field), pure (T := Fun (Lang.stack)) (vint 3)] ** 
+       ap_pointsto [("o": var), ("g" : field), pure (T := Fun (Lang.stack)) (vint 4)]) 
+      (ap_pointsto [("o": var), ("f": field), pure (T := Fun (Lang.stack)) (vint 3)] ** 
+      (ap_pointsto [("o": var), ("g": field), pure (T := Fun (Lang.stack)) (vint 4)]))
+      (cseq (cread "x" "o" "f") (cseq (cread "y" "o" "g") cskip)).                    
+Proof.
+  Time run_rtac reify_imp term_table (@runTac_sound rw_fail).
+Qed.
+
+Lemma test_write :
+	ltrue |--
+	triple
+      (ap_pointsto [("o": var), ("f" : field), pure (T := Fun (Lang.stack)) (vint 3)]) 
+      (ap_pointsto [("o": var), ("f": field), pure (T := Fun (Lang.stack)) (vint 4)])
+      (cseq (cwrite "o" "f" (E_val (vint 4))) cskip).                    
+Proof.
+  Time run_rtac reify_imp term_table (@runTac_sound rw_fail).
+Qed.
+
+Require Import BinInt.
+
+Fixpoint mkSwapPre n : sasn :=
+	match n with
+	  | 0   => empSP
+	  | S n => ap_pointsto [("o": Lang.var), (append "f" (nat2string10 n) : field), 
+	  	                     (eval (E_val (vint (Z.of_nat n))))] **
+	           mkSwapPre n
+	end.  
+
+	
+Fixpoint mkSwapPostAux n m :=
+  match n with
+    | 0 => empSP
+	| S n => ap_pointsto [("o": Lang.var), (append "f" (nat2string10 n) : field), 
+	  	                     (eval (E_val (vint (Z.of_nat (m - (S n))))))] **
+	         mkSwapPostAux n m
+  end.           
+  
+Definition mkSwapPost n := mkSwapPostAux n n.
+
+Fixpoint mkRead n c :=
+	match n with
+	  | 0 => c
+	  | S n => cseq (cread ((append "x" (nat2string10 n):Lang.var)) ("o":Lang.var) ((append "f" (nat2string10 n)):field))
+	                (mkRead n c)
+    end.
+						
+Fixpoint mkWriteAux n m c :=
+	match n with
+	  | 0 => c
+	  | S n => cseq (cwrite ("o":Lang.var) (append "f" (nat2string10 n)) (E_var (append "x" (nat2string10 (m - (S n))))))
+	                (mkWriteAux n m c)
+    end.
+
+Definition mkWrite n c := mkWriteAux n n c.
+
+Definition mkSwapProg (n : nat) (c : cmd) := mkRead n (mkWrite n c).
+	
+Definition mkSwap n :=
+	ltrue |-- triple (mkSwapPre n) (mkSwapPost n) (mkSwapProg n cskip).
+
+Set Printing Depth 100.
+
+  Opaque ap.
+
+Lemma test_swap : 
+|--
+( {[ap_pointsto  ["o", ("f")%string, eval (E_val (vint 5))] **
+    ap_pointsto  ["o", ("g")%string, eval (E_val (vint 6))] ** empSP]}
+ ("x")%string R= "o" [("f")%string];;
+ ("y")%string R= "o" [("g")%string];;
+ "o" [("f")%string] W= E_var ("y")%string;;
+ "o" [("g")%string] W=E_var ("x")%string;; Skip
+ {[ap_pointsto  ["o", ("f")%string, eval (E_val (vint 6))] **
+   ap_pointsto  ["o", ("g")%string, eval (E_val (vint 5))] ** empSP]} ).
+Proof.
+  Time run_rtac reify_imp term_table (@runTac_sound rw_fail).
+Qed.
+
+
+
+
+Lemma test_skip_lemma4 : testSkip 10.
+Proof.
+  unfold testSkip; simpl.
+  
+  Time run_rtac reify_imp term_table (@runTac_sound rw_fail).
+Time Qed.
+
+
+
+
+
+
+Print rtac_sound.
+Print rtac_spec.
+
+Lemma test_swap2 : mkSwap 40.
+Proof.
+  unfold mkSwap, mkSwapPre, mkSwapPost, mkSwapProg, mkSwapPostAux, mkRead, mkWrite, mkWriteAux.
+  
+  Time run_rtac reify_imp term_table (@runTac_sound rw_fail).
+Time Qed.
+
+
+
+
+
+
+
+
+
+
+
+
+
+
+
+
+
+
+
+
+
+
+
+
+
+
+
+
+
+
+
+
+
+
+
+
+
+
+
+
+
+
+
+
+
+
+
+
+
+
+
+
+
+
+
+
+End blurb.
+
+Instance EmptyEnv : Environment := {
+  java_env := SymEnv.from_list nil
+}.
+
+
+Definition ASSUMPTION : rtac typ (expr typ func) :=
+  EASSUMPTION (fun _ _ _ _ x y s => if x ?[ eq ] y then Some s else None).
+
+Lemma ASSUMPTION_sound : rtac_sound ASSUMPTION.
+Proof.
+  admit.
+Qed.
+
+Ltac rtac_derive_soundness :=
+  repeat first [ eapply IDTAC_sound
+               | eapply ASSUMPTION_sound
+               | eapply FAIL_sound
+               | eapply INSTANTIATE_sound
+               | eapply INTRO_sound
+               | eapply FIRST_sound ; Forall_rtac_derive_soundness
+               | eapply SOLVE_sound ; rtac_derive_soundness
+               | eapply THEN_sound ;
+                 [ rtac_derive_soundness
+                 | rtacK_derive_soundness ]
+               | eapply TRY_sound ; rtac_derive_soundness
+               | eapply REPEAT_sound ; rtac_derive_soundness
+               | eapply AT_GOAL_sound ; [ intros ; rtac_derive_soundness ]
+               | eapply APPLY_sound ; [ simpl ] (* TODO(gmalecha): Needs to change *)
+               | eapply EAPPLY_sound ; [ simpl ]  (* TODO(gmalecha): Needs to change *)
+               ]
+with rtacK_derive_soundness :=
+  first [ solve [eauto]
+        | eapply runOnGoals_sound ; rtac_derive_soundness
+        ]
+with Forall_rtac_derive_soundness :=
+  repeat first [ 
+                 eapply Forall_nil
+               | eapply Forall_cons ;
+                 [ try rtac_derive_soundness
+                 | try Forall_rtac_derive_soundness ] ].
+
+
+
+
+
+
+
+
+
+
+
+
+
+
+
+
+
+
+
+
+
+
+
+
+
+
+Lemma LTrue : True.
+Proof.
+  apply I.
+Qed.
+
+Definition true_lemma : lemma typ (expr typ func) (expr typ func).
+reify_lemma reify_imp LTrue.
+Defined.
+Print true_lemma.
+
+Lemma true_lemma_sound : 
+	lemmaD (exprD'_typ0 (T:=Prop)) nil nil true_lemma.
+Proof.
+  compute.
+  apply LTrue.
+Qed.
+
+Definition AUTO := APPLY typ func true_lemma.
+
+Lemma AUTO_sound : rtac_sound AUTO.
+Proof.
+  admit.
+Qed.
+
+Lemma test_true : True.
+Proof.
+  run_rtac reify_imp term_table AUTO_sound.
+Qed.
+  
+
+
+
+
+
+
+
+
+
+
+
+
+
+
+
+
+Lemma andI (P Q : Prop) (HP : P) (HQ : Q) : P /\ Q.
+Proof.
+  tauto.
+Qed.
+
+Definition andI_lemma : lemma typ (expr typ func) (expr typ func).
+Proof.
+  reify_lemma reify_imp andI.
+Defined.
+Print andI_lemma.
+Lemma andI_lemma_sound : 
+	lemmaD (exprD'_typ0 (T:=Prop)) nil nil andI_lemma.
+Proof.
+  compute. intros. apply andI. assumption. assumption.
+Qed.
+
+Definition AUTO' := 
+  THEN (REPEAT 10 (INTRO typ func)) 
+    (FIRST (THEN (APPLY typ func andI_lemma) ASSUMPTION ::
+      (APPLY typ func true_lemma) :: ASSUMPTION :: nil)).
+    
+Lemma AUTO'_sound : rtac_sound AUTO'.
+Proof.
+  unfold AUTO'.
+  rtac_derive_soundness.
+  admit.
+  admit.
+Qed.
+
+Lemma test_and : forall (P Q R : Prop), Q -> P -> R -> P /\ Q.
+Proof.
+  run_rtac reify_imp term_table AUTO'_sound.
+Qed.
+
+Print test_and.
+
+
+
+
+
+
+
+
+
+
+
+
+
+
+
+
+
+
+
+
+
+
+
+
+Lemma orI1 (P Q : Prop) (HP : P) : P \/ Q.
+Proof.
+  tauto.
+Qed.
+
+Lemma orI2 (P Q : Prop) (HQ : Q) : P \/ Q.
+Proof.
+  tauto.
+Qed.
+
+Definition orI1_lemma : lemma typ (expr typ func) (expr typ func).
+Proof.
+  reify_lemma reify_imp orI1.
+Defined.
+
+Definition orI2_lemma : lemma typ (expr typ func) (expr typ func).
+Proof.
+  reify_lemma reify_imp orI2.
+Defined.
+
+Lemma orI1_lemma_sound : 
+	lemmaD (exprD'_typ0 (T:=Prop)) nil nil orI1_lemma.
+Proof.
+  compute. intros. apply orI1. assumption.
+Qed.
+
+Lemma orI2_lemma_sound : 
+	lemmaD (exprD'_typ0 (T:=Prop)) nil nil orI1_lemma.
+Proof.
+  compute. intros. apply orI1. assumption.
+Qed.
+
+Definition AUTO'' := 
+  REC 20
+    (fun rec => THEN (REPEAT 10 (INTRO typ func)) 
+      (FIRST 
+        (THEN (APPLY typ func andI_lemma) rec ::
+        (THEN (APPLY typ func orI1_lemma) rec) ::
+        (THEN (APPLY typ func orI2_lemma) rec) ::
+        (APPLY typ func true_lemma) :: ASSUMPTION :: nil)))
+    FAIL.
+    
+Lemma AUTO''_sound : rtac_sound AUTO''.
+Proof.
+  unfold AUTO''.
+  (* rtac_derive_soundness. *)
+  admit.
+Qed.
+
+Lemma test_and2 : forall (P Q R T : Prop),
+	 Q -> P -> R -> (P /\ Q /\ R) \/
+	    (Q /\ T).
+Proof.
+  run_rtac reify_imp term_table AUTO''_sound.
+Qed.
